wip

Foundation/Modal/Hilbert2/Basic.lean
@@ -12,21 +12,32 @@ variable {α : Type*}
 structure Hilbert (α : Type*) where
   axioms : Set (Formula α)
 
-class Hilbert.FiniteAxiomatizable (H : Hilbert α) where
-  axioms_fin : Set.Finite H.axioms
+namespace Hilbert
 
 variable {H H₁ H₂ : Hilbert α}
 
-inductive Hilbert.Deduction (H : Hilbert α) : (Formula α) → Type _
-  | maxm {φ}      : φ ∈ H.axioms → Deduction H φ
+def axiomInstances (H : Hilbert α) : Set (Formula α) := { φ⟦s⟧ | (φ ∈ H.axioms) (s : Substitution α) }
+
+lemma mem_axiomInstances_of_mem_axioms {φ} (h : φ ∈ H.axioms) : φ ∈ H.axiomInstances := by
+  use φ;
+  constructor;
+  . assumption;
+  . use Substitution.id;
+    simp;
+
+class FiniteAxiomatizable (H : Hilbert α) where
+  axioms_fin : Set.Finite H.axioms := by aesop
+
+
+inductive Deduction (H : Hilbert α) : (Formula α) → Type _
+  | maxm {φ}      : φ ∈ H.axiomInstances → Deduction H φ
   | mdp {φ ψ}     : Deduction H (φ ➝ ψ) → Deduction H φ → Deduction H ψ
-  | subst {φ} (s) : Deduction H φ → Deduction H (φ⟦s⟧)
   | nec {φ}       : Deduction H φ → Deduction H (□φ)
   | imply₁ φ ψ    : Deduction H $ Axioms.Imply₁ φ ψ
   | imply₂ φ ψ χ  : Deduction H $ Axioms.Imply₂ φ ψ χ
   | ec φ ψ        : Deduction H $ Axioms.ElimContra φ ψ
 
-namespace Hilbert.Deduction
+namespace Deduction
 
 instance : System (Formula α) (Hilbert α) := ⟨Deduction⟩
 
@@ -42,192 +53,81 @@ instance : System.HasDiaDuality H := inferInstance
 
 instance : System.Necessitation H := ⟨nec⟩
 
-lemma maxm! {φ} (h : φ ∈ H.axioms) : H ⊢! φ := ⟨maxm h⟩
+lemma maxm! {φ} (h : φ ∈ H.axiomInstances) : H ⊢! φ := ⟨maxm h⟩
 
-lemma subst! {φ} (s) (h : H ⊢! φ) : H ⊢! φ⟦s⟧ := ⟨subst s h.some⟩
+end Deduction
 
-end Hilbert.Deduction
-
-
-namespace Hilbert
 
 open Deduction
 
 namespace Deduction
 
-variable {H : Hilbert α}
-
-noncomputable def inducition!
+noncomputable def rec!
   {motive      : (φ : Formula α) → H ⊢! φ → Sort*}
-  (hMaxm       : ∀ {φ}, (h : φ ∈ H.axioms) → motive φ ⟨maxm h⟩)
-  (hMdp        : ∀ {φ ψ}, {hpq : H ⊢! φ ➝ ψ} → {hp : H ⊢! φ} → motive (φ ➝ ψ) hpq → motive φ hp → motive ψ (mdp! hpq hp))
-  (hNec        : ∀ {φ}, {hp : H ⊢! φ} → (ihp : motive φ hp) → motive (□φ) (nec! hp))
-  (hSubst      : ∀ {φ} (s), {hp : H ⊢! φ} → (ihp : motive φ hp) → motive (φ⟦s⟧) (subst! s hp))
-  (hImply₁     : ∀ {φ ψ}, motive (Axioms.Imply₁ φ ψ) $ ⟨imply₁ φ ψ⟩)
-  (hImply₂     : ∀ {φ ψ χ}, motive (Axioms.Imply₂ φ ψ χ) $ ⟨imply₂ φ ψ χ⟩)
-  (hElimContra : ∀ {φ ψ}, motive (Axioms.ElimContra φ ψ) $ ⟨ec φ ψ⟩)
+  (maxm       : ∀ {φ}, (h : φ ∈ H.axiomInstances) → motive φ ⟨maxm h⟩)
+  (mdp        : ∀ {φ ψ}, {hpq : H ⊢! φ ➝ ψ} → {hp : H ⊢! φ} → motive (φ ➝ ψ) hpq → motive φ hp → motive ψ (mdp! hpq hp))
+  (nec        : ∀ {φ}, {hp : H ⊢! φ} → (ihp : motive φ hp) → motive (□φ) (nec! hp))
+  (imply₁     : ∀ {φ ψ}, motive (Axioms.Imply₁ φ ψ) $ ⟨imply₁ φ ψ⟩)
+  (imply₂     : ∀ {φ ψ χ}, motive (Axioms.Imply₂ φ ψ χ) $ ⟨imply₂ φ ψ χ⟩)
+  (ec : ∀ {φ ψ}, motive (Axioms.ElimContra φ ψ) $ ⟨ec φ ψ⟩)
   : ∀ {φ}, (d : H ⊢! φ) → motive φ d := by
   intro φ d;
   induction d.some with
-  | maxm h => exact hMaxm h
-  | mdp hpq hp ihpq ihp => exact hMdp (ihpq ⟨hpq⟩) (ihp ⟨hp⟩)
-  | nec hp ih => exact hNec (ih ⟨hp⟩)
-  | subst s hp ih => exact hSubst s (ih ⟨hp⟩)
+  | maxm h => exact maxm h
+  | mdp hpq hp ihpq ihp => exact mdp (ihpq ⟨hpq⟩) (ihp ⟨hp⟩)
+  | nec hp ih => exact nec (ih ⟨hp⟩)
   | _ => aesop;
+
+def subst! {φ} (s) (h : H ⊢! φ) : H ⊢! φ⟦s⟧ := by
+  induction h using Deduction.rec! with
+  | imply₁ => simp;
+  | imply₂ => simp;
+  | ec => simp;
+  | mdp ihφψ ihφ => exact ihφψ ⨀ ihφ;
+  | nec ihφ => exact nec! ihφ;
+  | maxm h =>
+    obtain ⟨ψ, h, ⟨s', rfl⟩⟩ := h;
+    apply maxm!;
+    use ψ;
+    constructor;
+    . assumption;
+    . use s' ∘ s;
+      exact subst_comp;
 
 end Deduction
 
-
-variable {H H₁ H₂ : Hilbert α}
 
 abbrev theorems (H : Hilbert α) := System.theory H
 
 lemma of_subset (hs : H₁.axioms ⊆ H₂.axioms) : H₁ ⊢! φ → H₂ ⊢! φ := by
   intro h;
-  induction h using Deduction.inducition! with
-  | hMaxm h => exact maxm! $ hs h;
-  | hMdp ih₁ ih₂ => exact mdp! ih₁ ih₂;
-  | hNec ih => exact nec! ih;
-  | hSubst s ih => exact subst! s ih;
+  induction h using Deduction.rec! with
+  | maxm h =>
+    obtain ⟨ψ, h, ⟨s, rfl⟩⟩ := h;
+    apply maxm!;
+    use ψ;
+    constructor;
+    . exact hs h;
+    . use s;
+  | mdp ih₁ ih₂ => exact mdp! ih₁ ih₂;
+  | nec ih => exact nec! ih;
+  | _ => simp;
+
+lemma weakerThan_of_dominate_axiomInstances (hMaxm : ∀ {φ : Formula α}, φ ∈ H₁.axiomInstances → H₂ ⊢! φ) : H₁ ≤ₛ H₂ := by
+  apply System.weakerThan_iff.mpr;
+  intro φ h;
+  induction h using Deduction.rec! with
+  | maxm h => apply hMaxm h;
+  | mdp ih₁ ih₂ => exact mdp! ih₁ ih₂;
+  | nec ih => exact nec! ih;
   | _ => simp;
 
 lemma weakerThan_of_dominate_axioms (hMaxm : ∀ {φ : Formula α}, φ ∈ H₁.axioms → H₂ ⊢! φ) : H₁ ≤ₛ H₂ := by
-  apply System.weakerThan_iff.mpr;
-  intro φ h;
-  induction h using Deduction.inducition! with
-  | hMaxm h => exact hMaxm h;
-  | hMdp ih₁ ih₂ => exact mdp! ih₁ ih₂;
-  | hNec ih => exact nec! ih;
-  | hSubst s ih => exact subst! s ih;
-  | _ => simp;
-
-lemma weakerThan_of_subset_axioms (hSubset : H₁.axioms ⊆ H₂.axioms) : H₁ ≤ₛ H₂ := by
-  apply weakerThan_of_dominate_axioms;
-  intro φ hp;
-  exact ⟨Deduction.maxm $ hSubset hp⟩;
+  apply weakerThan_of_dominate_axiomInstances;
+  rintro φ ⟨ψ, hψ, ⟨s, rfl⟩⟩;
+  apply subst!;
+  apply hMaxm hψ;
 
 end Hilbert
-
-
-
-namespace Hilbert
-
-def axiomInstances (H : Hilbert α) : Set (Formula α) := { φ⟦s⟧ | (φ ∈ H.axioms) (s : Substitution α) }
-
-lemma mem_axiomInstances_of_mem_axioms {φ} (h : φ ∈ H.axioms) : φ ∈ H.axiomInstances := by
-  use φ;
-  constructor;
-  . assumption;
-  . use Substitution.id;
-    simp;
-
-inductive Deduction₂ (H : Hilbert α) : (Formula α) → Type _
-  | maxm {φ}      : (φ ∈ H.axiomInstances) → Deduction₂ H φ
-  | mdp {φ ψ}     : Deduction₂ H (φ ➝ ψ) → Deduction₂ H φ → Deduction₂ H ψ
-  | nec {φ}       : Deduction₂ H φ → Deduction₂ H (□φ)
-  | imply₁ φ ψ    : Deduction₂ H $ Axioms.Imply₁ φ ψ
-  | imply₂ φ ψ χ  : Deduction₂ H $ Axioms.Imply₂ φ ψ χ
-  | ec φ ψ        : Deduction₂ H $ Axioms.ElimContra φ ψ
-
-notation H " ⊢² " φ => Deduction₂ H φ
-
-
-def Deductive₂ (H : Hilbert α) (φ) := Nonempty (H ⊢² φ)
-notation H " ⊢²! " φ => Deductive₂ H φ
-
-lemma Deduction₂.nec! {H : Hilbert α} {φ} (h : H ⊢²! φ) : H ⊢²! □φ := ⟨Deduction₂.nec h.some⟩
-
-
-noncomputable def Deduction₂.inducition!
-  {motive      : (φ : Formula α) → (H ⊢²! φ) → Sort*}
-  (hMaxm       : ∀ {φ}, (h : φ ∈ H.axiomInstances) → motive φ ⟨maxm h⟩)
-  (hMdp        : ∀ {φ ψ}, {hpq : H ⊢²! φ ➝ ψ} → {hp : H ⊢²! φ} → motive (φ ➝ ψ) hpq → motive φ hp → motive ψ ⟨mdp hpq.some hp.some⟩)
-  (hNec        : ∀ {φ}, {hp : H ⊢²! φ} → (ihp : motive φ hp) → motive (□φ) ⟨nec hp.some⟩)
-  (hImply₁     : ∀ {φ ψ}, motive (Axioms.Imply₁ φ ψ) $ ⟨imply₁ φ ψ⟩)
-  (hImply₂     : ∀ {φ ψ χ}, motive (Axioms.Imply₂ φ ψ χ) $ ⟨imply₂ φ ψ χ⟩)
-  (hElimContra : ∀ {φ ψ}, motive (Axioms.ElimContra φ ψ) $ ⟨ec φ ψ⟩)
-  : ∀ {φ}, (d : H ⊢²! φ) → motive φ d := by
-  intro φ d;
-  induction d.some with
-  | maxm h => exact hMaxm h
-  | mdp hpq hp ihpq ihp => exact hMdp (ihpq ⟨hpq⟩) (ihp ⟨hp⟩)
-  | nec hp ih => exact hNec (ih ⟨hp⟩)
-  | _ => aesop;
-
-
-lemma deductive₂_of_deductive : H ⊢! φ → H ⊢²! φ := by
-  intro h;
-  induction h using Deduction.inducition! with
-  | hMaxm h => exact ⟨Deduction₂.maxm (mem_axiomInstances_of_mem_axioms (by assumption))⟩;
-  | hMdp ih₁ ih₂ => exact ⟨Deduction₂.mdp ih₁.some ih₂.some⟩;
-  | hNec ih => exact ⟨Deduction₂.nec ih.some⟩;
-  | @hSubst φ s h₁ h₂ => sorry;
-    /-
-    obtain ⟨d₂⟩ := h₂;
-    constructor;
-    cases d₂;
-    . sorry;
-    . sorry;
-    . sorry;
-    . apply Deduction₂.imply₁;
-    . apply Deduction₂.imply₂;
-    . apply Deduction₂.ec;
-    -/
-  | hImply₁ => exact ⟨Deduction₂.imply₁ _ _⟩;
-  | hImply₂ => exact ⟨Deduction₂.imply₂ _ _ _⟩;
-  | hElimContra => exact ⟨Deduction₂.ec _ _⟩;
-
-lemma deductive_of_deductive₂ : (H ⊢²! φ) → (H ⊢! φ) := by
-  intro h;
-  induction h using Deduction₂.inducition! with
-  | hMaxm h =>
-    obtain ⟨ψ, h, ⟨s, rfl⟩⟩ := h;
-    exact Deduction.subst! s $ Deduction.maxm! h;
-  | hMdp ih₁ ih₂ => exact ih₁ ⨀ ih₂;
-  | hNec ih => exact nec! ih;
-  | _ => simp;
-
-theorem iff_deductive_deductive₂ : H ⊢! φ ↔ H ⊢²! φ := ⟨deductive₂_of_deductive, deductive_of_deductive₂⟩
-
-end Hilbert
-
-
-/-
-namespace Hilbert
-
-def Deduction.isSubstless : H ⊢ φ → Prop
-  | subst _ _ => False
-  | _ => True
-
-def SubstlessDeduction (H : Hilbert α) (φ : Formula α) := { d : H ⊢ φ // Deduction.isSubstless d }
-notation H " ⊢ˢ " φ => SubstlessDeduction H φ
-
-open Deduction in
-noncomputable def SubstlessDeduction.rec {motive : Formula α → Sort*}
-  {motive      : (φ : Formula α) → (H ⊢ˢ φ) → Sort*}
-  (hMdp        : ∀ {φ ψ}, {hpq : H ⊢ˢ (φ ➝ ψ)} → {hp : H ⊢ˢ φ} → motive (φ ➝ ψ) hpq → motive φ hp → motive ψ ⟨.mdp hpq.1 hp.1, by simp [isSubstless]⟩)
-  (hNec        : ∀ {φ}, {hp : H ⊢ˢ φ} → (ihp : motive φ hp) → motive (□φ) ⟨.nec hp.1, by simp [isSubstless]⟩)
-  (hImply₁     : ∀ {φ ψ}, motive (φ ➝ ψ ➝ φ) $ ⟨imply₁ φ ψ, by simp [isSubstless]⟩)
-  (hImply₂     : ∀ {φ ψ χ}, motive ((φ ➝ ψ ➝ χ) ➝ (φ ➝ ψ) ➝ φ ➝ χ) $ ⟨imply₂ φ ψ χ, by simp [isSubstless]⟩)
-  (hElimContra : ∀ {φ ψ}, motive (Axioms.ElimContra φ ψ) $ ⟨ec φ ψ, by simp [isSubstless]⟩)
-  : ∀ {φ}, (d : H ⊢ˢ φ) → motive φ d := by
-  rintro φ ⟨d, hd⟩;
-  induction d with
-  | subst s hp ih => simp [isSubstless] at hd;
-  -- | maxm h => exact hMaxm h
-  -- | mdp hpq hp ihpq ihp => exact hMdp (ihpq ⟨hpq⟩) (ihp ⟨hp⟩)
-  | @nec ψ hp ih =>
-    have := ih ?_;
-    have := @hNec ψ;
-    sorry;
-    . sorry;
-  | _ => sorry;
-  -- | _ => aesop;
-
-def SubstlessDeductive (H : Hilbert α) (φ) := Nonempty (SubstlessDeduction H φ)
-notation H:90 " ⊢ˢ! " φ:90 => SubstlessDeductive H φ
-
-end Hilbert
--/
 
 end LO.Modal
