Foundation/Modal/Kripke2/Definability.lean
@@ -6,9 +6,17 @@ namespace Kripke
 
 variable {C : Kripke.FrameClass}
 
-def FrameClass.definedBy (C : Kripke.FrameClass) (Γ : Set (Formula ℕ)) := ∀ F, F ∈ C ↔ (∀ φ ∈ Γ, F ⊧ φ)
 
-def FrameClass.definedByFormula (C : Kripke.FrameClass) (φ : Formula ℕ) := C.definedBy {φ}
+class FrameClass.DefinedBy (C : Kripke.FrameClass) (Γ : Set (Formula ℕ)) where
+  defines : ∀ F, F ∈ C ↔ (∀ φ ∈ Γ, F ⊧ φ)
+
+class FrameClass.FiniteDefinedBy (C Γ) extends FrameClass.DefinedBy C Γ where
+  finite : Set.Finite Γ
+
+class FrameClass.IsNonempty (C : Kripke.FrameClass) where
+  nonempty : Nonempty C
+
+-- def FrameClass.definedByFormula (C : Kripke.FrameClass) (φ : Formula ℕ) := C.definedBy {φ}
 
 
 -- lemma subst_instances (definedBy : C.definedBy Γ) (h : φ ∈ Γ) : ∀ s, F ⊧ φ  := by sorry;
