Foundation/Modal/Hilbert2/K.lean
@@ -11,27 +11,26 @@ section
 class HasK (H : Hilbert α) where
   p : α
   q : α
-  ne_pq : p ≠ q
+  ne_pq : p ≠ q := by trivial;
   mem_K : Axioms.K (.atom p) (.atom q) ∈ H.axioms := by tauto;
 
 instance [DecidableEq α] [hK : H.HasK] : System.HasAxiomK H where
   K φ ψ := by
-    simpa [hK.ne_pq] using
-      subst (s := λ b => if hK.p = b then φ else if hK.q = b then ψ else (.atom b)) $
-      maxm hK.mem_K;
+    apply maxm;
+    use Axioms.K (.atom hK.p) (.atom hK.q);
+    constructor;
+    . exact hK.mem_K;
+    . use (λ b => if hK.p = b then φ else if hK.q = b then ψ else (.atom b));
+      simp [hK.ne_pq];
 
 end
 
 
 section
 
-protected def K : Hilbert ℕ := ⟨{Axioms.K (.atom 0) (.atom 1)}⟩
-
-instance : (Hilbert.K).HasK where
-  p := 0
-  q := 1
-  ne_pq := by trivial;
-
+protected abbrev K : Hilbert ℕ := ⟨{Axioms.K (.atom 0) (.atom 1)}⟩
+instance : Hilbert.K.FiniteAxiomatizable where
+instance : Hilbert.K.HasK where p := 0; q := 1
 instance : System.K (Hilbert.K) where
 
 end
