Foundation/Modal/Hilbert2/WellKnown.lean
@@ -17,23 +17,39 @@ class HasT (H : Hilbert α) where
   mem_T : Axioms.T (.atom p) ∈ H.axioms := by tauto;
 
 instance [hT : H.HasT] : System.HasAxiomT H where
-  T φ := by simpa using subst (s := λ b => if hT.p = b then φ else (.atom b)) $ maxm hT.mem_T;
-
+  T φ := by
+    apply maxm;
+    use Axioms.T (.atom hT.p);
+    constructor;
+    . exact hT.mem_T;
+    . use (λ b => if hT.p = b then φ else (.atom b));
+      simp;
 
 class HasB (H : Hilbert α) where
   p : α
   mem_B : Axioms.B (.atom p) ∈ H.axioms := by tauto;
 
 instance [hB : H.HasB] : System.HasAxiomB H where
-  B φ := by simpa using subst (s := λ b => if hB.p = b then φ else (.atom b)) $ maxm hB.mem_B;
-
+  B φ := by
+    apply maxm;
+    use Axioms.B (.atom hB.p);
+    constructor;
+    . exact hB.mem_B;
+    . use (λ b => if hB.p = b then φ else (.atom b));
+      simp;
 
 class HasD (H : Hilbert α) where
   p : α
   mem_D : Axioms.D (.atom p) ∈ H.axioms := by tauto;
 
 instance [hD : H.HasD] : System.HasAxiomD H where
-  D φ := by simpa using subst (s := λ b => if hD.p = b then φ else (.atom b)) $ maxm hD.mem_D;
+  D φ := by
+    apply maxm;
+    use Axioms.D (.atom hD.p);
+    constructor;
+    . exact hD.mem_D;
+    . use (λ b => if hD.p = b then φ else (.atom b));
+      simp;
 
 
 class HasFour (H : Hilbert α) where
@@ -41,7 +57,13 @@ class HasFour (H : Hilbert α) where
   mem_Four : Axioms.Four (.atom p) ∈ H.axioms := by tauto;
 
 instance [hFour : H.HasFour] : System.HasAxiomFour H where
-  Four φ := by simpa using subst (s := λ b => if hFour.p = b then φ else (.atom b)) $ maxm hFour.mem_Four;
+  Four φ := by
+    apply maxm;
+    use Axioms.Four (.atom hFour.p);
+    constructor;
+    . exact hFour.mem_Four;
+    . use (λ b => if hFour.p = b then φ else (.atom b));
+      simp;
 
 
 class HasFive (H : Hilbert α) where
@@ -49,7 +71,13 @@ class HasFive (H : Hilbert α) where
   mem_Five : Axioms.Five (.atom p) ∈ H.axioms := by tauto;
 
 instance [hFive : H.HasFive] : System.HasAxiomFive H where
-  Five φ := by simpa using subst (s := λ b => if hFive.p = b then φ else (.atom b)) $ maxm hFive.mem_Five;
+  Five φ := by
+    apply maxm;
+    use Axioms.Five (.atom hFive.p);
+    constructor;
+    . exact hFive.mem_Five;
+    . use (λ b => if hFive.p = b then φ else (.atom b));
+      simp;
 
 
 class HasDot2 (H : Hilbert α) where
@@ -57,20 +85,29 @@ class HasDot2 (H : Hilbert α) where
   mem_Dot2 : Axioms.Dot2 (.atom p) ∈ H.axioms := by tauto;
 
 instance [hDot2 : H.HasDot2] : System.HasAxiomDot2 H where
-  Dot2 φ := by simpa using subst (s := λ b => if hDot2.p = b then φ else (.atom b)) $ maxm hDot2.mem_Dot2;
+  Dot2 φ := by
+    apply maxm;
+    use Axioms.Dot2 (.atom hDot2.p);
+    constructor;
+    . exact hDot2.mem_Dot2;
+    . use (λ b => if hDot2.p = b then φ else (.atom b));
+      simp;
 
 
 class HasDot3 (H : Hilbert α) where
   p : α
   q : α
-  ne_pq : p ≠ q
+  ne_pq : p ≠ q := by trivial;
   mem_Dot3 : Axioms.Dot3 (.atom p) (.atom q) ∈ H.axioms := by tauto;
 
 instance [hDot3 : H.HasDot3] : System.HasAxiomDot3 H where
   Dot3 φ ψ := by
-    simpa [hDot3.ne_pq] using
-      subst (s := λ b => if hDot3.p = b then φ else if hDot3.q = b then ψ else (.atom b)) $
-      maxm hDot3.mem_Dot3;
+    apply maxm;
+    use Axioms.Dot3 (.atom hDot3.p) (.atom hDot3.q);
+    constructor;
+    . exact hDot3.mem_Dot3;
+    . use (λ b => if hDot3.p = b then φ else if hDot3.q = b then ψ else (.atom b));
+      simp [hDot3.ne_pq];
 
 
 class HasL (H : Hilbert α) where
@@ -78,7 +115,13 @@ class HasL (H : Hilbert α) where
   mem_L : Axioms.L (.atom p) ∈ H.axioms := by tauto;
 
 instance [hL : H.HasL] : System.HasAxiomL H where
-  L φ := by simpa using subst (s := λ b => if hL.p = b then φ else (.atom b)) $ maxm hL.mem_L;
+  L φ := by
+    apply maxm;
+    use Axioms.L (.atom hL.p);
+    constructor;
+    . exact hL.mem_L;
+    . use (λ b => if hL.p = b then φ else (.atom b));
+      simp;
 
 
 class HasGrz (H : Hilbert α) where
@@ -86,7 +129,13 @@ class HasGrz (H : Hilbert α) where
   mem_Grz : Axioms.Grz (.atom p) ∈ H.axioms := by tauto;
 
 instance [hGrz : H.HasGrz] : System.HasAxiomGrz H where
-  Grz φ := by simpa using subst (s := λ b => if hGrz.p = b then φ else (.atom b)) $ maxm hGrz.mem_Grz;
+  Grz φ := by
+    apply maxm;
+    use Axioms.Grz (.atom hGrz.p);
+    constructor;
+    . exact hGrz.mem_Grz;
+    . use (λ b => if hGrz.p = b then φ else (.atom b));
+      simp;
 
 
 class HasTc (H : Hilbert α) where
@@ -94,7 +143,13 @@ class HasTc (H : Hilbert α) where
   mem_Tc : Axioms.Tc (.atom p) ∈ H.axioms := by tauto;
 
 instance [hTc : H.HasTc] : System.HasAxiomTc H where
-  Tc φ := by simpa using subst (s := λ b => if hTc.p = b then φ else (.atom b)) $ maxm hTc.mem_Tc;
+  Tc φ := by
+    apply maxm;
+    use Axioms.Tc (.atom hTc.p);
+    constructor;
+    . exact hTc.mem_Tc;
+    . use (λ b => if hTc.p = b then φ else (.atom b));
+      simp;
 
 
 class HasVer (H : Hilbert α) where
@@ -102,60 +157,66 @@ class HasVer (H : Hilbert α) where
   mem_Ver : Axioms.Ver (.atom p) ∈ H.axioms := by tauto;
 
 instance [DecidableEq α] [hVer : H.HasVer] : System.HasAxiomVer H where
-  Ver φ := by simpa using subst (s := λ b => if hVer.p = b then φ else (.atom b)) $ maxm hVer.mem_Ver;
+  Ver φ := by
+    apply maxm;
+    use Axioms.Ver (.atom hVer.p);
+    constructor;
+    . exact hVer.mem_Ver;
+    . use (λ b => if hVer.p = b then φ else (.atom b));
+      simp;
 
 end
 
 
 protected abbrev Ver : Hilbert ℕ := ⟨{Axioms.K (.atom 0) (.atom 1), Axioms.Ver (.atom 0)}⟩
-instance : (Hilbert.Ver).HasK where p := 0; q := 1; ne_pq := by trivial
+instance : (Hilbert.Ver).HasK where p := 0; q := 1;
 instance : (Hilbert.Ver).HasVer where p := 0
 
 
 protected abbrev Triv : Hilbert ℕ := ⟨{ Axioms.K (.atom 0) (.atom 1), Axioms.T (.atom 0), Axioms.Tc (.atom 0)}⟩
-instance : (Hilbert.Triv).HasK where p := 0; q := 1; ne_pq := by trivial;
+instance : (Hilbert.Triv).HasK where p := 0; q := 1;
 instance : (Hilbert.Triv).HasT where p := 0
 instance : (Hilbert.Triv).HasTc where p := 0
 
 
 protected abbrev K4 : Hilbert ℕ := ⟨{Axioms.K (.atom 0) (.atom 1), Axioms.Four (.atom 0)}⟩
-instance : (Hilbert.K4).HasK where p := 0; q := 1; ne_pq := by trivial
+instance : (Hilbert.K4).HasK where p := 0; q := 1;
 instance : (Hilbert.K4).HasFour where p := 0
 
 
 protected abbrev S4 : Hilbert ℕ := ⟨{Axioms.K (.atom 0) (.atom 1), Axioms.T (.atom 0), Axioms.Four (.atom 0)}⟩
-instance : (Hilbert.S4).HasK where p := 0; q := 1; ne_pq := by trivial
+instance : (Hilbert.S4).HasK where p := 0; q := 1;
 instance : (Hilbert.S4).HasT where p := 0
 instance : (Hilbert.S4).HasFour where p := 0
 
 
 protected abbrev S4Dot2 : Hilbert ℕ := ⟨{Axioms.K (.atom 0) (.atom 1), Axioms.T (.atom 0), Axioms.Four (.atom 0), Axioms.Dot2 (.atom 0)}⟩
-instance : (Hilbert.S4Dot2).HasK where p := 0; q := 1; ne_pq := by trivial
+instance : (Hilbert.S4Dot2).HasK where p := 0; q := 1;
 instance : (Hilbert.S4Dot2).HasT where p := 0
 instance : (Hilbert.S4Dot2).HasFour where p := 0
 instance : (Hilbert.S4Dot2).HasDot2 where p := 0
 
 
 protected abbrev S4Dot3 : Hilbert ℕ := ⟨{Axioms.K (.atom 0) (.atom 1), Axioms.T (.atom 0), Axioms.Four (.atom 0), Axioms.Dot3 (.atom 0) (.atom 1)}⟩
-instance : (Hilbert.S4Dot3).HasK where p := 0; q := 1; ne_pq := by trivial
+instance : (Hilbert.S4Dot3).HasK where p := 0; q := 1;
 instance : (Hilbert.S4Dot3).HasT where p := 0
 instance : (Hilbert.S4Dot3).HasFour where p := 0
-instance : (Hilbert.S4Dot3).HasDot3 where p := 0; q := 1; ne_pq := by trivial
+instance : (Hilbert.S4Dot3).HasDot3 where p := 0; q := 1;
 
 
 protected abbrev S5 : Hilbert ℕ := ⟨{Axioms.K (.atom 0) (.atom 1), Axioms.T (.atom 0), Axioms.Five (.atom 0)}⟩
-instance : (Hilbert.S5).HasK where p := 0; q := 1; ne_pq := by trivial
+instance : (Hilbert.S5).HasK where p := 0; q := 1;
 instance : (Hilbert.S5).HasT where p := 0
 instance : (Hilbert.S5).HasFive where p := 0
 
 
 protected abbrev GL : Hilbert ℕ := ⟨{Axioms.K (.atom 0) (.atom 1), Axioms.L (.atom 0)}⟩
-instance : (Hilbert.GL).HasK where p := 0; q := 1; ne_pq := by trivial
+instance : (Hilbert.GL).HasK where p := 0; q := 1;
 instance : (Hilbert.GL).HasL where p := 0
 
 
 protected abbrev Grz : Hilbert ℕ := ⟨{Axioms.K (.atom 0) (.atom 1), Axioms.Grz (.atom 0)}⟩
-instance : (Hilbert.Grz).HasK where p := 0; q := 1; ne_pq := by trivial
+instance : (Hilbert.Grz).HasK where p := 0; q := 1;
 instance : (Hilbert.Grz).HasGrz where p := 0
 
 
