Foundation/Modal/Kripke2/Completeness.lean
@@ -1,0 +1,197 @@
+import Foundation.Modal.MaximalConsistentSet
+import Foundation.Modal.Kripke2.Basic
+
+namespace LO.Modal
+
+open System
+open Formula
+open Kripke
+open MaximalConsistentSet
+
+variable {S} [System (Formula ℕ) S]
+variable {𝓢 : S} [System.Consistent 𝓢] [System.K 𝓢]
+
+namespace Kripke
+
+abbrev canonicalFrame (𝓢 : S) [System.Consistent 𝓢] [System.K 𝓢] : Kripke.Frame where
+  World := MCS 𝓢
+  Rel X Y := □''⁻¹X.1 ⊆ Y.1
+
+namespace canonicalFrame
+
+variable {Ω₁ Ω₂ : (canonicalFrame 𝓢).World}
+
+@[simp] lemma rel_def_box: Ω₁ ≺ Ω₂ ↔ ∀ {φ}, □φ ∈ Ω₁ → φ ∈ Ω₂ := by simp [Frame.Rel']; aesop;
+
+lemma multirel_def_multibox : Ω₁ ≺^[n] Ω₂ ↔ ∀ {φ}, □^[n]φ ∈ Ω₁.1 → φ ∈ Ω₂.1 := by
+  induction n generalizing Ω₁ Ω₂ with
+  | zero =>
+    simp_all only [Rel.iterate.iff_zero, Function.iterate_zero, id_eq];
+    constructor;
+    . intro h; tauto_set;
+    . intro h;
+      apply intro_equality;
+      tauto_set;
+  | succ n ih =>
+    constructor;
+    . intro h φ hp;
+      obtain ⟨⟨Ω₃, _⟩, R₁₃, R₃₂⟩ := h;
+      apply ih.mp R₃₂ $ rel_def_box.mp R₁₃ (by simpa using hp);
+    . intro h;
+      obtain ⟨Ω, hΩ⟩ := lindenbaum (𝓢 := 𝓢) (T := (□''⁻¹Ω₁.1 ∪ ◇''^[n]Ω₂.1)) $ by
+        apply FormulaSet.intro_union_consistent;
+        rintro Γ Δ ⟨hΓ, hΔ⟩ hC;
+
+        replace hΓ : ∀ φ ∈ Γ, □φ ∈ Ω₁ := by simpa using hΓ;
+        have dΓconj : Ω₁.1 *⊢[𝓢]! □⋀Γ := membership_iff.mp $ iff_mem_box_conj.mpr hΓ;
+
+        have hΔ₂ : ∀ φ ∈ ◇'⁻¹^[n]Δ, φ ∈ Ω₂ := by
+          intro φ hp;
+          exact Set.iff_mem_multidia.mp $ hΔ (◇^[n]φ) (by simpa using hp);
+
+        have hΔconj : ⋀◇'⁻¹^[n]Δ ∈ Ω₂ := iff_mem_conj.mpr hΔ₂;
+
+        have : ⋀◇'⁻¹^[n]Δ ∉ Ω₂ := by {
+          have d₁ : 𝓢 ⊢! ⋀Γ ➝ ⋀Δ ➝ ⊥ := and_imply_iff_imply_imply'!.mp hC;
+          have : 𝓢 ⊢! ⋀(◇'^[n]◇'⁻¹^[n]Δ) ➝ ⋀Δ := by
+            apply conjconj_subset!;
+            intro ψ hq;
+            obtain ⟨χ, _, _⟩ := hΔ ψ hq;
+            subst_vars;
+            simpa;
+          have : 𝓢 ⊢! ◇^[n]⋀◇'⁻¹^[n]Δ ➝ ⋀Δ := imp_trans''! iff_conjmultidia_multidiaconj! $ this;
+          have : 𝓢 ⊢! ∼(□^[n](∼⋀◇'⁻¹^[n]Δ)) ➝ ⋀Δ := imp_trans''! (and₂'! multidia_duality!) this;
+          have : 𝓢 ⊢! ∼⋀Δ ➝ □^[n](∼⋀◇'⁻¹^[n]Δ) := contra₂'! this;
+          have : 𝓢 ⊢! (⋀Δ ➝ ⊥) ➝ □^[n](∼⋀◇'⁻¹^[n]Δ) := imp_trans''! (and₂'! neg_equiv!) this;
+          have : 𝓢 ⊢! ⋀Γ ➝ □^[n](∼⋀◇'⁻¹^[n]Δ) := imp_trans''! d₁ this;
+          have : 𝓢 ⊢! □⋀Γ ➝ □^[(n + 1)](∼⋀◇'⁻¹^[n]Δ) := by simpa using imply_box_distribute'! this;
+          exact iff_mem_neg.mp $ h $ membership_iff.mpr $ (Context.of! this) ⨀ dΓconj;
+        }
+
+        contradiction;
+      use Ω;
+      constructor;
+      . intro φ hp;
+        apply hΩ;
+        simp_all;
+      . apply ih.mpr;
+        apply multibox_multidia.mpr;
+        intro φ hp;
+        apply hΩ;
+        simp_all;
+
+lemma multirel_def_multibox' : Ω₁ ≺^[n] Ω₂ ↔ ∀ {φ}, φ ∈ (□''⁻¹^[n]Ω₁.1) → φ ∈ Ω₂.1 := by
+  constructor;
+  . intro h φ hp; exact multirel_def_multibox.mp h hp;
+  . intro h; apply multirel_def_multibox.mpr; assumption;
+
+lemma multirel_def_multidia : Ω₁ ≺^[n] Ω₂ ↔ ∀ {φ}, (φ ∈ Ω₂.1 → ◇^[n]φ ∈ Ω₁.1) := Iff.trans multirel_def_multibox multibox_multidia
+
+lemma rel_def_dia : Ω₁ ≺ Ω₂ ↔ ∀ {φ}, φ ∈ Ω₂.1 → ◇φ ∈ Ω₁.1 := by simpa using multirel_def_multidia (n := 1) (Ω₁ := Ω₁) (Ω₂ := Ω₂)
+
+end canonicalFrame
+
+
+abbrev canonicalModel (𝓢 : S) [System.Consistent 𝓢] [System.K 𝓢] : Model where
+  toFrame := canonicalFrame 𝓢
+  Val Ω a := (atom a) ∈ Ω.1
+
+@[reducible]
+instance : Semantics (Formula ℕ) (canonicalModel 𝓢).World := Formula.Kripke.Satisfies.semantics (M := canonicalModel 𝓢)
+
+
+section lemmata
+
+variable {φ ψ : Formula ℕ}
+
+lemma truthlemma : ∀ {Ω : (canonicalModel 𝓢).World}, Ω ⊧ φ ↔ (φ ∈ Ω.1) := by
+  induction φ using Formula.rec' with
+  | hatom => simp_all [Semantics.Realize, Kripke.Satisfies];
+  | hfalsum =>
+    simp only [Semantics.Realize, Satisfies, false_iff];
+    exact not_mem_falsum;
+  | hbox φ ih =>
+    intro Ω;
+    constructor;
+    . intro h;
+      apply iff_mem_box.mpr;
+      intro Ω' hΩ';
+      apply ih.mp;
+      exact h Ω' hΩ';
+    . intro h Ω' hΩ';
+      apply ih.mpr;
+      exact canonicalFrame.rel_def_box.mp hΩ' h;
+  | himp φ ψ ihp ihq =>
+    intro Ω;
+    constructor;
+    . intro h;
+      apply iff_mem_imp.mpr;
+      intro hp; replace hp := ihp.mpr hp;
+      exact ihq.mp $ h hp;
+    . intro h;
+      have := iff_mem_imp.mp h;
+      intro hp; replace hp := ihp.mp hp;
+      exact ihq.mpr $ this hp
+
+
+lemma iff_valid_on_canonicalModel_deducible : (canonicalModel 𝓢) ⊧ φ ↔ 𝓢 ⊢! φ := by
+  constructor;
+  . contrapose;
+    intro h;
+    have : FormulaSet.Consistent 𝓢 ({∼φ}) := by
+      apply FormulaSet.def_consistent.mpr;
+      intro Γ hΓ;
+      by_contra hC;
+      have : 𝓢 ⊢! φ := dne'! $ neg_equiv'!.mpr $ replace_imply_left_conj! hΓ hC;
+      contradiction;
+    obtain ⟨Ω, hΩ⟩ := lindenbaum this;
+    apply not_validOnModel_of_exists_world;
+    use Ω;
+    exact truthlemma.not.mpr $ iff_mem_neg.mp (by tauto_set);
+  . intro h Ω;
+    suffices φ ∈ Ω.1 by exact truthlemma.mpr this;
+    by_contra hC;
+    obtain ⟨Γ, hΓ₁, hΓ₂⟩ := FormulaSet.iff_insert_inconsistent.mp $ (MaximalConsistentSet.maximal' hC);
+    have : Γ ⊢[𝓢]! ⊥ := FiniteContext.provable_iff.mpr $ and_imply_iff_imply_imply'!.mp hΓ₂ ⨀ h;
+    have : Γ ⊬[𝓢] ⊥ := FormulaSet.def_consistent.mp (MaximalConsistentSet.consistent) _ hΓ₁;
+    contradiction;
+
+/-
+lemma realize_axiomset_of_self_canonicalModel : (canonicalModel 𝓢) ⊧* H.axioms := by
+  apply Semantics.realizeSet_iff.mpr;
+  intro φ hp;
+  apply iff_valid_on_canonicalModel_deducible.mpr;
+  exact maxm! hp;
+
+lemma realize_theory_of_self_canonicalModel : (canonicalModel 𝓢) ⊧* (System.1 H) := by
+  apply Semantics.realizeSet_iff.mpr;
+  intro φ hp;
+  apply iff_valid_on_canonicalModel_deducible.mpr;
+  simpa [System.1] using hp;
+-/
+
+lemma complete_of_canonical {C : FrameClass} (hFC : canonicalFrame 𝓢 ∈ C) : C ⊧ φ → 𝓢 ⊢! φ := by
+  contrapose;
+  intro h;
+  apply not_validOnFrameClass_of_exists_model;
+  use (canonicalModel 𝓢);
+  constructor;
+  . assumption;
+  . exact iff_valid_on_canonicalModel_deducible.not.mpr h;
+
+lemma instCompleteOfCanonical {C : FrameClass} (hC : (Kripke.canonicalFrame 𝓢) ∈ C) : Complete 𝓢 C := ⟨complete_of_canonical hC⟩
+
+end lemmata
+
+end Kripke
+
+
+/-
+namespace K
+
+instance Kripke.complete : Complete (Hilbert.K ℕ) (Kripke.AllFrameClass) := Hilbert.Kripke.instCompleteOfCanonical (C := Kripke.AllFrameClass) $ by tauto
+
+end K
+-/
+
+end LO.Modal
