Foundation/Modal/Kripke2/Hilbert/K.lean
@@ -1,0 +1,21 @@
+import Foundation.Modal.Hilbert2.K
+import Foundation.Modal.Kripke2.Hilbert.Soundness
+import Foundation.Modal.Kripke2.Completeness
+
+namespace LO.Modal
+
+instance : Kripke.AllFrameClass.DefinedBy (Hilbert.K.axiomInstances) := ⟨by
+  suffices ∀ F, ∀ φ ∈ Hilbert.K.axiomInstances, Formula.Kripke.ValidOnFrame F φ by simpa;
+  rintro F _ ⟨ψ, ⟨_, rfl⟩, ⟨s, rfl⟩⟩;
+  apply Formula.Kripke.ValidOnFrame.axiomK;
+⟩
+
+namespace Hilbert.K
+
+instance : System.Consistent (Hilbert.K) := Kripke.Hilbert.instConsistent (C := Kripke.AllFrameClass) ⟨⟨Fin 1, λ _ _ => True⟩, by trivial⟩
+
+instance : Complete (Hilbert.K) (Kripke.AllFrameClass) := Kripke.instCompleteOfCanonical trivial
+
+end Hilbert.K
+
+end LO.Modal
